Integrate typing predicates into OPERATORS layer

Interface.v
@@ -18,7 +18,6 @@ Module Export Op <: OPERATORS.
   Definition val: Type := Values.val.
 
   Inductive type' : Type :=
-  | Tbool:  type'
   | Tint:   Ctypes.intsize -> Ctypes.signedness -> type'
   | Tlong:  Ctypes.signedness -> type'
   | Tfloat: Ctypes.floatsize -> type'.
@@ -27,7 +26,6 @@ Module Export Op <: OPERATORS.
 
   Definition cltype (ty: type) : Ctypes.type :=
     match ty with
-    | Tbool      => Ctypes.type_bool
     | Tint sz sg => Ctypes.Tint sz sg Ctypes.noattr
     | Tlong sg   => Ctypes.Tlong sg Ctypes.noattr
     | Tfloat sz  => Ctypes.Tfloat sz Ctypes.noattr
@@ -47,7 +45,7 @@ Module Export Op <: OPERATORS.
   Lemma true_not_false_val: true_val <> false_val.
   Proof. discriminate. Qed.
 
-  Definition bool_type : type := Tbool.
+  Definition bool_type : type := Tint Ctypes.IBool Ctypes.Signed.
 
   Inductive constant : Type :=
   | Cint: Integers.int -> Ctypes.intsize -> Ctypes.signedness -> constant
@@ -67,10 +65,10 @@ Module Export Op <: OPERATORS.
 
   Definition sem_const (c: const) : val :=
     match c with
-    | Cint i _ _ => Values.Vint i
-    | Clong i _  => Values.Vlong i
-    | Cfloat f   => Values.Vfloat f
-    | Csingle f  => Values.Vsingle f
+    | Cint i sz sg => Values.Vint (Cop.cast_int_int sz sg i)
+    | Clong i sg   => Values.Vlong i
+    | Cfloat f     => Values.Vfloat f
+    | Csingle f    => Values.Vsingle f
     end.
 
   Inductive unop' : Type :=
@@ -108,6 +106,225 @@ Module Export Op <: OPERATORS.
     | Errors.OK ty' => typecl ty'
     | Errors.Error _ => None
     end.
+
+  (* Neither Vundef nor Vptr is well-typed.
+
+     In CompCert's Ctyping, we have:
+       forall ty, wt_val Vundef ty
+
+     Allowing that, in particular, values read from uninitialized
+     memory are well-typed. Our typing invariants become slightly more
+     complicated -- they will require that variables be initialized before
+     they are read -- but also slightly stronger, since we need not treat
+     the Vundef case.
+  *)
+  Inductive wt_val' : val -> type -> Prop :=
+  | wt_val_int:
+      forall n sz sg,
+        Ctyping.wt_int n sz sg ->
+        wt_val' (Values.Vint n) (Tint sz sg)
+  | wt_val_long:
+      forall n sg,
+        wt_val' (Values.Vlong n) (Tlong sg)
+  | wt_val_float:
+      forall f,
+        wt_val' (Values.Vfloat f) (Tfloat Ctypes.F64)
+  | wt_val_single:
+      forall f,
+        wt_val' (Values.Vsingle f) (Tfloat Ctypes.F32).
+
+  Definition wt_val : val -> type -> Prop := wt_val'.
+
+  Lemma wt_val_true:
+    wt_val true_val bool_type.
+  Proof.
+    apply wt_val_int.
+    reflexivity.
+  Qed.
+
+  Lemma wt_val_false:
+    wt_val false_val bool_type.
+  Proof.
+    apply wt_val_int.
+    reflexivity.
+  Qed.
+
+  Lemma wt_val_const:
+    forall c, wt_val (sem_const c) (type_const c).
+  Proof.
+    destruct c.
+    - apply wt_val_int. apply Ctyping.pres_cast_int_int.
+    - apply wt_val_long.
+    - apply wt_val_float.
+    - apply wt_val_single.
+  Qed.
+
+  Lemma typecl_wt_val_wt_val:
+    forall cty ty v,
+      typecl cty = Some ty ->
+      Ctyping.wt_val v cty ->
+      v <> Values.Vundef ->
+      (forall b ofs, v <> Values.Vptr b ofs) ->
+      wt_val v ty.
+  Proof.
+    intros ** Htcl Hcty Hnun Hnptr.
+    destruct cty; try discriminate;
+      (destruct a; destruct attr_volatile; destruct attr_alignas;
+       try discriminate; simpl in *; fold Ctypes.noattr in Hcty).
+    - injection Htcl; intro HR; rewrite HR in *; clear Htcl.
+      rewrite <-HR; clear HR.
+      destruct v; try now inversion Hcty.
+      + now contradiction Hnun.
+      + inversion_clear Hcty. now apply wt_val_int.
+      + exfalso; now eapply Hnptr.
+    - injection Htcl; intro HR; rewrite HR in *; clear Htcl.
+      rewrite <-HR; clear HR.
+      destruct v; try now inversion Hcty.
+      + now contradiction Hnun.
+      + now apply wt_val_long.
+    - injection Htcl; intro HR; rewrite HR in *; clear Htcl.
+      rewrite <-HR; clear HR.
+      destruct v; try now inversion Hcty.
+      + now contradiction Hnun.
+      + destruct f; try now inversion Hcty.
+        now apply wt_val_float.
+      + destruct f; try now inversion Hcty.
+        now apply wt_val_single.
+  Qed.
+
+  Lemma wt_val_not_vundef_nor_vptr:
+    forall v ty,
+      wt_val v ty ->
+      v <> Values.Vundef /\ (forall b ofs, v <> Values.Vptr b ofs).
+  Proof.
+    intros ** Hwt.
+    destruct ty; inversion Hwt; subst;
+      split; discriminate.
+  Qed.
+
+  Lemma wt_val_wt_val_cltype:
+    forall v ty,
+      wt_val v ty ->
+      Ctyping.wt_val v (cltype ty).
+  Proof.
+    intros ** Hwt.
+    destruct ty; inversion_clear Hwt.
+    - now apply Ctyping.wt_val_int.
+    - now apply Ctyping.wt_val_long.
+    - now apply Ctyping.wt_val_float.
+    - now apply Ctyping.wt_val_single.
+  Qed.
+
+  Lemma pres_sem_unop:
+    forall op ty1 ty v1 v,
+      type_unop op ty1 = Some ty ->
+      sem_unop op v1 ty1 = Some v ->
+      wt_val v1 ty1 ->
+      wt_val v ty.
+  Proof.
+    intros ** Htop Hsop Hv1.
+    pose proof (wt_val_not_vundef_nor_vptr _ _ Hv1) as [Hnun Hnptr].
+    destruct op as [uop|].
+    - (* UnaryOp *)
+      simpl in *.
+      destruct (Ctyping.type_unop uop (cltype ty1)) as [cty|] eqn:Hok;
+        [|discriminate].
+      pose proof (Ctyping.pres_sem_unop _ _ _ _ _ _ Hok Hsop
+                                        (wt_val_wt_val_cltype _ _ Hv1)) as Hcwt.
+      clear Hok.
+      cut (v <> Values.Vundef /\ (forall b ofs, v <> Values.Vptr b ofs)).
+      destruct 1 as (Hnun' & Hnptr');
+        now apply typecl_wt_val_wt_val with (1:=Htop); eauto.
+      destruct uop; simpl in *.
+      + rewrite Cop.notbool_bool_val in Hsop.
+        destruct (Cop.bool_val v1 (cltype ty1) Memory.Mem.empty);
+          try discriminate.
+        injection Hsop; intro; subst v.
+        destruct b; simpl; split; discriminate.
+      + unfold Cop.sem_notint in Hsop.
+          destruct (Cop.classify_notint (cltype ty1));
+            destruct v1; try discriminate;
+            injection Hsop; intro; subst; split; discriminate.
+      + unfold Cop.sem_neg in Hsop.
+        destruct (Cop.classify_neg (cltype ty1));
+          destruct v1; try discriminate;
+          injection Hsop; intro; subst; split; discriminate.
+      + unfold Cop.sem_absfloat in Hsop.
+        destruct (Cop.classify_neg (cltype ty1));
+          destruct v1; try discriminate;
+            injection Hsop; intro; subst; split; discriminate.
+    - (* CastOp *)
+      (* TODO: automate proof on the example of Ctyping.pres_sem_cast *)
+      simpl in Hsop. simpl in Htop.
+      destruct (Ctyping.check_cast (cltype ty1) (cltype t));
+        [|discriminate].
+      destruct ty1 as [i1 s1|s1|f1];
+        destruct t as [i2 s2|s2|f2];
+        injection Htop; intro; subst; simpl in Hsop;
+          destruct v1 as [i|i|f|f|b|ofs]; inversion_clear Hv1.
+      + destruct i, i1, s1, i2, s2; inversion_clear Hsop;
+          try (apply wt_val_int; simpl;
+               try (rewrite Int.sign_ext_idem||rewrite Int.zero_ext_idem);
+               intuition);
+          match goal with |- context [if ?c then _ else _] => destruct c end;
+          auto.
+      + destruct i, i1, s1, s2; inversion_clear Hsop; apply wt_val_long.
+      + destruct i, i1, s1, f2; inversion_clear Hsop;
+          (apply wt_val_single || apply wt_val_float).
+      + destruct f, s1, i2, s2; inversion_clear Hsop;
+          try (apply wt_val_int; simpl;
+               try (rewrite Int.sign_ext_idem||rewrite Int.zero_ext_idem);
+               intuition);
+          match goal with |- context [if ?c then _ else _] => destruct c end;
+          auto.
+      + destruct f, s1; inversion_clear Hsop; apply wt_val_long.
+      + destruct f, s1, f2; inversion_clear Hsop;
+          (apply wt_val_single || apply wt_val_float).
+      + unfold Cop.sem_cast in Hsop.
+        destruct f1, i2, s2; simpl in Hsop; try discriminate;
+          (destruct (Float.to_int f) || destruct (Float.to_intu f));
+          try (destruct (Float.to_intu f));
+          try discriminate;
+          injection Hsop; intro; subst; apply wt_val_int; simpl;
+          try ((rewrite Int.sign_ext_idem||rewrite Int.zero_ext_idem);
+               now intuition);
+          try match goal with |- context [if ?c then _ else _] => destruct c end;
+          auto.
+      + unfold Cop.sem_cast in Hsop.
+        destruct f1, i2, s2; simpl in Hsop; try discriminate;
+          (destruct (Float32.to_int b) || destruct (Float32.to_intu b));
+          try (destruct (Float32.to_intu b));
+          try discriminate;
+          injection Hsop; intro; subst; apply wt_val_int; simpl;
+          try ((rewrite Int.sign_ext_idem||rewrite Int.zero_ext_idem);
+               now intuition);
+          try match goal with |- context [if ?c then _ else _] => destruct c end;
+          auto.
+      + apply Cop.cast_val_is_casted in Hsop;
+          inversion_clear Hsop.
+        apply wt_val_long.
+      + apply Cop.cast_val_is_casted in Hsop;
+          inversion_clear Hsop.
+        apply wt_val_long.
+      + apply Cop.cast_val_is_casted in Hsop;
+          inversion_clear Hsop.
+        now apply wt_val_float.
+        now apply wt_val_single.
+      + apply Cop.cast_val_is_casted in Hsop;
+          inversion_clear Hsop.
+        now apply wt_val_float.
+        now apply wt_val_single.
+  Qed.
+
+  Lemma pres_sem_binop:
+    forall op ty1 ty2 ty v1 v2 v,
+      type_binop op ty1 ty2 = Some ty ->
+      sem_binop op v1 ty1 v2 ty2 = Some v ->
+      wt_val v1 ty1 ->
+      wt_val v2 ty2 ->
+      wt_val v ty.
+  Proof.
+  Admitted.
 
   Lemma val_dec   : forall v1 v2 : val, {v1 = v2} + {v1 <> v2}.
   Proof Values.Val.eq.
